Fixes(?) mistakes on the definitions for the functions dec_is_flattened and flatten. Made flatten way more simple, so proving its termination can be done with just the fun command instead of function.

Syntax.thy
@@ -9,11 +9,9 @@ datatype ach = Unin | AC | Hom
 locale signature =
   fixes arity :: "'f \<Rightarrow> nat"
     and label :: "'f \<Rightarrow> ach"
-  assumes label_inj: "inj label"
 
 begin
 
-(* baby lemmas about labels *)
 lemma non_ac : 
   assumes \<open>label f \<noteq> AC\<close>
   shows \<open>label f = Unin \<or> label f = Hom\<close>
@@ -21,61 +19,35 @@ using ach.exhaust assms by blast
 
 section \<open>Flattened Terms\<close>
 
-text \<open>blabla \<close>
+inductive is_flattened :: "('f, 'v) term \<Rightarrow> bool" where
+  var_is_flattened:
+    "is_flattened (Var x)" |
 
+  fun_is_flattened:
+    "\<lbrakk> label f \<noteq> AC; \<And>t. t \<in> set ts \<Longrightarrow> is_flattened t \<rbrakk> \<Longrightarrow> is_flattened (Fun f ts)" |
 
-inductive IsFlattened :: "('f, 'v) term \<Rightarrow> bool" where
-  varIsFlattened:
-    "IsFlattened (Var x)" |
-
-  funIsFlattened:
-    "\<lbrakk> label f \<noteq> AC;
-       \<And>t. t \<in> set ts \<Longrightarrow> IsFlattened t \<rbrakk>
-     \<Longrightarrow> IsFlattened (Fun f ts)" |
-
-  acIsFlattened:
+  ac_is_flattened:
     "\<lbrakk> label f = AC;
-       \<And>t. t \<in> set ts \<Longrightarrow> IsFlattened t;
-       \<And>t g tss. t \<in> set ts \<Longrightarrow> t = Fun g tss \<Longrightarrow> g \<noteq> f \<rbrakk>
-     \<Longrightarrow> IsFlattened (Fun f ts)"
+       \<And>t. t \<in> set ts \<Longrightarrow> is_flattened t;
+       \<And>t g gs. t \<in> set ts \<Longrightarrow> t = Fun g gs \<Longrightarrow> g \<noteq> f \<rbrakk>  \<Longrightarrow> is_flattened (Fun f ts)"
 
-(*
-
-Is_Flattened t1 \<and> Is_Flattened t2 \<and> Is_Flattened t3 \<and> head(ti)\<noteq> f
-------------------------------------------------------------------- f=AC
-Is_flattened f[t1,t2,t3]
-*)
-lemma test1_IsFlattened:
+lemma test1_is_flattened:
   assumes "label f = Unin"
-  shows "IsFlattened (Fun f [Var x, Fun f [Var y, Var x]])"
-  by (metis ach.simps(2) assms empty_set funIsFlattened list.simps(15) set_ConsD singletonD
-      varIsFlattened)
+  shows "is_flattened (Fun f [Var x, Fun f [Var y, Var x]])"
+  by (metis ach.simps(2) assms empty_set fun_is_flattened list.simps(15) set_ConsD singletonD
+      var_is_flattened)
 
 
-lemma test2_IsFlattened:
+lemma test2_is_flattened:
   assumes "label f = AC"
-  shows "\<not> IsFlattened (Fun f [Var x, Fun f [Var y, Var x]])"
-  using assms signature.IsFlattened.cases signature_axioms by force
- 
- 
-(*
-lemma test1_IsFlattened:
-  assumes "label f = AC" and "label g = Hom"
-  shows "\<not>(IsFlattened (Fun f [Var x, Fun g [Var y, Fun f [Var z, Fun f [Var z, Var x]]]]))"
-  sorry 
+  shows "\<not> is_flattened (Fun f [Var x, Fun f [Var y, Var x]])"
+  using assms signature.is_flattened.cases by force
 
-  
-lemma test2_IsFlattened:
-  assumes "label f = AC" and "label g = Hom"
-  shows "IsFlattened (Fun f [Var x, Fun g [Var y, Fun f [Var z, Fun f [Var z, Var x]]]])"
-   sorry
-
-*)
 value  "set [Var x, Fun g [Fun f [Var y, Var x], Var x]]"
 
 lemma example2:
   assumes "label f = AC" and "label g = Unin"
-  shows "IsFlattened (Fun f [Var x, Fun g [Fun f [Var y, Var x], Var x]])"
+  shows "is_flattened (Fun f [Var x, Fun g [Fun f [Var y, Var x], Var x]])"
   sorry
 
 (* Now we define a function that decides the above predicate *)
@@ -86,13 +58,12 @@ fun is_headed_by_ac :: \<open>('f, 'v) term \<Rightarrow> bool\<close> where
       (Var _)   \<Rightarrow> False |
       (Fun g _) \<Rightarrow> (case label g of
         AC \<Rightarrow> True |
-        _ \<Rightarrow> False)
-  )\<close>
-
+        _  \<Rightarrow> False)
+    )\<close>
 
 lemma test_is_headed_by_ac:
   assumes "label f = AC" and "label g = Unin"
-  shows "is_headed_by_ac (Fun f [Var x, Fun g [Var y, Var z]])"
+  shows "is_headed_by_ac (Fun f [Var x, Fun f [Var y, Var z]])"
   using assms by simp
 
 lemma test_is_not_headed_by_ac:
@@ -108,236 +79,168 @@ proof
 qed
 
 
-fun dec_IsFlattened :: \<open>('f, 'v) term \<Rightarrow> bool\<close> where
-  \<open>dec_IsFlattened (Var _) = True\<close> |
-  \<open>dec_IsFlattened (Fun f ts) =
+fun get_fun_symb :: \<open>('f, 'v) term \<Rightarrow> 'f option \<close> where
+  \<open>get_fun_symb (Var _ )  = None\<close> |
+  \<open>get_fun_symb (Fun f _) = Some f\<close>
+
+lemma isVar_None: "isVar s \<longleftrightarrow> get_fun_symb s = None"
+  sorry
+
+fun dec_is_flattened :: \<open>('f, 'v) term \<Rightarrow> bool\<close> where
+  \<open>dec_is_flattened (Var _) = True\<close> |
+  \<open>dec_is_flattened (Fun f ts) =
     (case label f of
       AC \<Rightarrow> (
-        let ac_arg = find is_headed_by_ac ts in
+        let ac_arg =
+          find
+            (\<lambda> s. (is_headed_by_ac s) \<and> (case (get_fun_symb s) of None \<Rightarrow> False | Some g \<Rightarrow> f = g))
+            ts
+        in
         (case ac_arg of
-          None \<Rightarrow> True |
+          None \<Rightarrow> foldl (\<and>) True (map dec_is_flattened ts) |
           Some _ \<Rightarrow> False)
-      )|
-      _  \<Rightarrow> foldl (\<and>) True (map dec_IsFlattened ts)
+    )|
+      _  \<Rightarrow> foldl (\<and>) True (map dec_is_flattened ts)
     )\<close>
 
+(*
+Note:
+ 1. The repeated "foldl (\<and>) True (map dec_is_flattened ts)" is for efficiency reasons, we only compute
+  this foldl when strictly necessary, that's why there is no let ... in construct computing it
+  beforehand, as some branches of the function wouldn't need it.
+ 2. Notice that on Line 105, there is no way that (is_headed_by_ac s) is true and the second component is false.
+    Since to be headed by AC you need to be of functional application form.
+    I cannot express this at the type level and Isabelle doesn't seem to subscribe to the "propositions as types" idea.
+*)
 
-lemma test_dec_IsFlattened:
+lemma test_dec_is_flattened:
   assumes "label f = AC"
-  shows "\<not> dec_IsFlattened (Fun f [Var x, Fun f [Var y, Var z]])"
+  shows "\<not> dec_is_flattened (Fun f [Var x, Fun f [Var y, Var z]])"
   using assms by simp
 
 text \<open> The following should not be possible to prove. \<close>
-lemma test1_dec_IsFlattened:
+lemma test1_dec_is_flattened:
   assumes "label f = AC" and "label g = Hom"
-  shows " dec_IsFlattened (Fun f [Var x, Fun g [Var y, Fun f [Var z, Fun f [Var z, Var x]]]])"
+  shows " dec_is_flattened (Fun f [Var x, Fun g [Var y, Fun f [Var z, Fun f [Var z, Var x]]]])"
   apply (auto)
   apply (simp add: assms)
-  done 
+  sorry
 
 lemma dec_pred_flatten:
-  assumes "IsFlattened s"
-  shows " dec_IsFlattened s"
+  assumes "is_flattened s"
+  shows " dec_is_flattened s"
   apply (induction s)
    apply (simp)
   sorry
 
 lemma dec_pred_is_flatten:
-  "IsFlattened s \<longleftrightarrow> dec_IsFlattened s" (is "?L \<longleftrightarrow> ?R ")
+  "is_flattened s \<longleftrightarrow> dec_is_flattened s" (is "?L \<longleftrightarrow> ?R ")
   sorry
 
 (*proof (cases s)
   case (Var x)
   then show ?thesis
-    using Var varIsFlattened by fastforce
+    using Var var_is_flattened by fastforce
 next
 case (Fun f ts)
   then show ?thesis
   proof
-    assume H: "IsFlattened (Fun f ts)"
+    assume H: "is_flattened (Fun f ts)"
     from H show ?thesis
-      unfolding dec_IsFlattened_def
+      unfolding dec_is_flattened_def
     proof (cases "label f = AC")
       case True
-      (* AC case: use your acIsFlattened rule / elimination to match
-         the condition that dec_IsFlattened checks for AC-symbols *)
+      (* AC case: use your ac_is_flattened rule / elimination to match
+         the condition that dec_is_flattened checks for AC-symbols *)
       from H True show ?thesis
-        by (auto elim: IsFlattened.cases)
+        by (auto elim: is_flattened.cases)
     next
       case False
-      (* non-AC case: use funIsFlattened + IH on all arguments *)
+      (* non-AC case: use fun_is_flattened + IH on all arguments *)
       from H False show ?thesis
-        by (auto elim: IsFlattened.cases)
+        by (auto elim: is_flattened.cases)
     qed
   next
-    assume H: "dec_IsFlattened (Fun f ts)"
-    show "IsFlattened (Fun f ts)"
-      unfolding dec_IsFlattened_def
+    assume H: "dec_is_flattened (Fun f ts)"
+    show "is_flattened (Fun f ts)"
+      unfolding dec_is_flattened_def
     proof (cases "label f = AC")
       case True
-      (* AC case: build an IsFlattened proof using acIsFlattened *)
+      (* AC case: build an is_flattened proof using ac_is_flattened *)
       from H True show ?thesis
-        by (auto intro: IsFlattened.intros)
+        by (auto intro: is_flattened.intros)
     next
       case False
-      (* non-AC case: use funIsFlattened and IH on arguments *)
+      (* non-AC case: use fun_is_flattened and IH on arguments *)
       from H False show ?thesis
-        by (auto intro: IsFlattened.intros)
+        by (auto intro: is_flattened.intros)
     qed
   qed
 qed
 *)
-(*
 
-This function is too complicated, the implementation above is simpler.
-Leaving the old one here to compare. Deleate it on next commit.
-
-fun dec_is_flatten_aux :: \<open>('f, 'v) term \<Rightarrow> bool \<Rightarrow> bool\<close> where
-  (* \<open>dec_is_flatten_aux (Var _) True = False\<close>  | *)
-  \<open>dec_is_flatten_aux (Var _) _ = True\<close>   |
-  \<open>dec_is_flatten_aux (Fun f ts) False =
-    (case (label f) of
-      AC \<Rightarrow> foldl (\<and>) True (map (\<lambda> t. dec_is_flatten_aux t True) ts)|
-      _ \<Rightarrow>  foldl (\<and>) True (map (\<lambda> t. dec_is_flatten_aux t False) ts)
-    )\<close> |
-  \<open>dec_is_flatten_aux (Fun f ts) True =
-    (case (label f) of
-      AC \<Rightarrow> False |
-      _  \<Rightarrow> foldl (\<and>) True (map (\<lambda> t. dec_is_flatten_aux t False) ts)
-    )\<close>
-
-fun dec_is_flatten :: \<open>('f, 'v) term \<Rightarrow> bool\<close> where
-  \<open>dec_is_flatten t = dec_is_flatten_aux t False\<close>
-
-
-+ [s1 , ..., sm ]
-
-  1. 
-
-
-*)
 
 text \<open>We define a function that flattens a term\<close>
 
-fun pred_split_aux :: \<open>('a \<Rightarrow> bool) \<Rightarrow> 'a list \<Rightarrow> 'a list * 'a list \<Rightarrow> 'a list * 'a list\<close> where
-  \<open>pred_split_aux P xs (ys,ns)=
-    (case xs of
-      []      \<Rightarrow> (ys,ns) |
-      x # xs' \<Rightarrow> (
-        if P x then 
-          pred_split_aux P xs' (x#ys, ns)
-        else
-          pred_split_aux P xs' (ys, x#ns)
+fun flatten_aux :: \<open>'f \<Rightarrow> ('f, 'v) term \<Rightarrow> ('f, 'v) term list\<close> where
+  \<open>flatten_aux f s =
+  (case s of
+    Var _ \<Rightarrow> [s] |
+    Fun g ss \<Rightarrow> (
+      (if label g = AC \<and> g = f then
+        args s
+      else
+        [s]
       )
-    )\<close>
-
-fun pred_split :: \<open>('a \<Rightarrow> bool) \<Rightarrow> 'a list \<Rightarrow> 'a list * 'a list\<close> where
-  \<open>pred_split P xs = pred_split_aux P xs ([],[])\<close>
+    )
+  )
+  \<close>
 
 fun flatten :: \<open>('f, 'v) term \<Rightarrow> ('f, 'v) term\<close> where
-  \<open>flatten s = 
+  \<open>flatten s =
     (case s of
       Var _    \<Rightarrow> s |
       Fun f ss \<Rightarrow>
         (case label f of
-          AC \<Rightarrow> (
-            let args_split = pred_split is_headed_by_ac ss in
-            let ac_args  = fst args_split in
-            let nac_args = snd args_split in
-            (case ac_args of
-              []    \<Rightarrow> s |
-              _ # _ \<Rightarrow> (
-                let args_of_ac_args = concat (map args ac_args) in
-                Fun f (args_of_ac_args @ nac_args)
-              )
-            )
-        )|
+          AC \<Rightarrow>
+          (
+            let flatten_all_args = map flatten ss in
+            let new_args = concat (map (flatten_aux f) flatten_all_args) in
+            Fun f new_args
+          )|
           _  \<Rightarrow> Fun f (map flatten ss)
         )
     )\<close>
 
-text \<open>O exemplo abaixo está com problema \<close>
+section \<open>Lemmata for Flatten\<close>
 
-lemma test1_Flatten:
-  assumes "label f = AC" and "label g = Hom"
-  shows " flatten (Fun f [Var x, Fun g [Var y, Fun f [Var z, Fun f [Var z, Var x]]]]) = Fun f [Var x, Fun g [Var y, Fun f [Var z, Var z, Var x]]] "
-  apply (simp add: assms)
-  sorry
-
-lemma flatten_soundness: \<open>\<forall> t::('f, 'v) term. IsFlattened (flatten t)\<close>
+lemma flatten_soundness: \<open>\<forall> t::('f, 'v) term. is_flattened (flatten t)\<close>
   sorry
 
 (* or *)
 
-lemma flatten_soundness_dec: \<open>\<forall> t::('f, 'v) term. dec_IsFlattened t \<close>
+lemma flatten_soundness_dec: \<open>\<forall> t::('f, 'v) term. dec_is_flattened (flatten t)\<close>
   sorry
 
+text \<open>O exemplo abaixo está com problema, agora esta certo\<close>
 
-(* I think this function is correct in the sense of the lemmas above.
-  However, i think it is still wrong: 
-  notice that we only check for those arguments that are labelled with AC without ever
-  discriminating them apart, and we put all together...
-  this will cause flatten to change the semantics of the term whenever the
-  input signature have more than one symbol labelled as AC.
+lemma test1_Flatten:
+  assumes "label f = AC" and "label g = Hom"
+  shows "flatten (Fun f [Var z, Fun f [Var x, Var y]]) = Fun f [Var z, Var x, Var y]"
+  apply (simp add: assms)
+  done
 
-  Mean Spirited Example:
-  Let \<Sigma> be f : AC, and g : AC, (other symbols can be added...
+(* now this example and more complicated ones also work.
+  but to prove more complicated ones, one need to be able to correctly do the ordering.
+  - There is an interesting lemma in AC_equality.thy that says:
+  \<forall>s. ac_eq (flatten s) s, that is, every term is equal to its flattened form modulo AC.
+ *)
 
-  So flatten of s = f [t1 ; ..., g [s1,s2] , ...., g [s3, s4] , ... , tn) will compute as follows:
-
-  ac_args = [ g[s1,s2] , g [s3, s4] ] (so we collected all AC arguments of s), 
-  the non ac arguments are on the other list
-
-  args_of_ac_args = [ [s1, s2] , [s3, s4] ] (collect all the arguments of the AC terms)
-
-  then we flatten the list
-
-  args_of_ac_args = [s1, s2, s3, s4 ]
-
-  later we combine them back into the arguments of s
-
-  flatten s = f [s1 , s2 , s3 , s4] @ [t1, ...., tn ]
-
-  now see that g function symbol disappeared...
-
-  BUT according to our relation IsFlattened flatten s is flat, which is actually correct
-
-  but s above is not flat...
-
-  if we consider a signature that has more than one ac symbol:
-      s = f [t1 ; ..., g [s1,s2] , ...., g [s3, s4] , ... , tn)
-      is flattened, (assuming f doesn't occur in the t_is for simplicity's sake)
-
-      so IsFlattened MUST be defined with respect to the same function symbol
-      not only the labels.
-
-      This way, s is flattened because none of 
-      its direct arguments are labelled AC AND are headed by f
-
-      
-
-Questions then:
-  1. Can our ACh (or even the AC from maximal) algorithm deal with more than one AC symbol?
-    - Intuitively, it can as long as we can dinamically change the label of a symbol.
-    - But i am not sure if this was even considered by guilherme when defining the ACh unification.
-    
-
-Possible approaches:
-  1. We restrict the whole formalization and terms to a single AC constructor.
-    - Functions must change, but that's fine since we are earlier in the definitions.
-    - The predicate IsFlattened and flatten function doesn't change
-
-  2. We keep it general and allow for multiple AC symbols.
-    - Then we need to change IsFlattened and flatten.
-    - I don't think anything changes on the definition of equality since there we enforce
-    that two functions headed by function symbol are equal only if their head symbols are equal.
-
-I like 2 more, specially if the original paper only considered a single AC symbol... 
-We can say we have a general ACh unification that is also formalized :)
-
-I am taking this decision alone so discussions are needed.
-
-*)
-
+text \<open>This one is not possible because of the variable ordering\<close>
+lemma test2_Flatten:
+  assumes "label f = AC" and "label g = Hom"
+  shows "flatten (Fun f [Var z, Fun f [Var x, Var y]]) = Fun f [Var x, Var y, Var y]"
+  apply (simp add: assms)
+  sorry
 end
 end
